upd

coqimp/ext/finaltheorem.v
@@ -27,15 +27,82 @@ Unset Strict Implicit.
 Open Scope code_scope.
 Open Scope mem_scope.
 
+CoInductive IdxEtrace {tprog} (step : tprog -> msg -> tprog -> Prop): Index -> tprog -> Etr -> Prop :=
+| IdxEtr_tau1 : forall P P' P'' idx idx',
+    star_tau_step step P P' -> step P' tau P'' ->
+    IdxEtrace step idx' P'' empEtr -> IdxEtrace step idx P empEtr
+| IdxEtr_tau2 : forall P P' idx idx',
+    star_tau_step step P P' -> idx' ⩹ idx ->
+    IdxEtrace step idx' P' empEtr -> IdxEtrace step idx P empEtr
+| IdxEtr_abort : forall P P' m idx,
+    star_tau_step step P P' -> (~ (exists P'', step P' m P'')) -> IdxEtrace step idx P abortEtr
+| Etr_event : forall P P' P'' v etr idx idx',
+    star_tau_step step P P' -> step P' (out v) P'' ->
+    IdxEtrace step idx' P'' etr -> IdxEtrace step idx P (outEtr v etr).
+
+(*
 Inductive n_tau_step {prog : Type} (step : prog -> msg -> prog -> Prop) :
   Index -> prog -> prog -> Prop :=
-| Zero_tau_step : forall p idx, n_tau_step step idx p p
-| Multi_tau_step : forall (p p' p'' : prog) idx_i idx_j,
-    step p tau p' -> idx_j ⩹ idx_i -> n_tau_step step idx_j p' p'' -> 
-    n_tau_step step idx_i p p''.
+| Zero_tau_step : forall p idx, ~ (exists idx', idx' ⩹ idx) -> n_tau_step step idx p p
+| Multi_tau_step : forall (p p' p'' p''': prog) idx_i idx_j,
+    star_tau_step step p p' -> step p' tau p'' -> idx_j ⩹ idx_i ->
+    n_tau_step step idx_j p'' p''' -> 
+    n_tau_step step idx_i p p'''.
+
+Lemma Etr_emp_n_step :
+  forall A (P : A) ndx (step : A -> msg -> A -> Prop),
+    Etrace step P empEtr -> well_founded LtIndex ->
+    exists P', n_tau_step step ndx P P'.
+Proof.
+  intros.
+  generalize dependent P.
+  generalize dependent step.
+  unfold well_founded in H0.
+  specialize (H0 ndx).
+  induction H0; intros.
+  inv H1.
+  destruct x.
+  destruct n, n0.
+  {
+    exists P.
+    eapply Zero_tau_step.
+    intro.
+    destruct H1.
+    inv H1; try omega.
+  }
+  {
+    eapply H0 in H4; eauto.
+    Focus 2.
+    instantiate (1 := (0%nat, n0)); econstructor; eauto.
+    destruct H4 as [P''' H4].
+    exists P'''.
+    eapply Multi_tau_step; eauto.
+    econstructor; eauto.
+  }
+  {
+    eapply H0 in H4; eauto.
+    Focus 2.
+    instantiate (1 := (n, 0%nat)); econstructor; eauto.
+    destruct H4 as [P''' H4].
+    exists P'''.
+    eapply Multi_tau_step; eauto.
+    econstructor; eauto.
+  }
+  {
+    eapply H0 in H4; eauto.
+    Focus 2.
+    instantiate (1 := (S n, n0)).
+    econstructor; eauto.
+    destruct H4 as [P''' H4].
+    exists P'''.
+    eapply Multi_tau_step; eauto.
+    econstructor; eauto.
+  }
+Qed.
 
 Lemma LEtr_emp_n_step_H_progress :
   forall LP LP' HP ndx idx,
+    well_founded LtIndex ->
     n_tau_step LP__ ndx LP LP' -> wp_sim idx LP HP -> idx ⩹ ndx ->
     (exists HP' HP'', star_step HP__ HP HP' /\ HP__ HP' tau HP'').
 Proof.
@@ -43,6 +110,75 @@ Proof.
   generalize dependent LP.
   generalize dependent LP'.
   generalize dependent HP.
+  generalize dependent idx.
+  unfold well_founded in H. 
+  specialize (H ndx).
+  induction H; intros.
+  inv H1.
+  contradiction H4; eauto.
+  inv H3.
+  clear H8 H9.
+  inv H4.
+  {
+    eapply H1 in H5.
+    clear H1.
+    destruct H5.
+    {
+      destruct H1 as [idx1 [Hlt Hwp_sim] ].
+      eapply H0 in Hwp_sim.
+      eauto.
+      instantiate(1 := idx); eauto.
+      eauto.
+      
+    }
+  }
+  
+  generalize dependent HP.
+  generalize dependent idx.
+  induction H; intros.
+  contradiction H; eauto.
+  inv H4. 
+  clear H6 H7.
+  
+  
+  induction H1; intros.
+  {
+    inv H0.
+    false.
+    contradiction H2.
+    exists (n, m').
+    econstructor; eauto.
+    Print Index.
+  }
+ *)
+
+Lemma wp_sim_ensures_refinement' :
+  forall C Cas S pc npc PrimSet HS B idx,
+    C ⊥ Cas -> wp_sim idx (C ⊎ Cas, (S, pc, npc)) (C, PrimSet, HS) ->
+    Etrace LP__ (C ⊎ Cas, (S, pc, npc)) B ->
+    IdxEtrace HP__ idx (C, PrimSet, HS) B.
+Proof.
+  cofix Hp; intros.
+  destruct B.
+  {
+    inv H1.
+    inv H2.
+    {
+      inv H0. 
+      clear H2 H5.
+      lets Hlp_step : H3.
+      eapply H1 in H3; eauto.
+      clear H1.
+      destruct H3 as [ [idx1 [Hlt H3] ] | [idx1 [ HP' [HP'' [Hstar [HPstep Hwpsim] ] ] ] ] ].
+      {
+        eapply IdxEtr_tau2.
+        instantiate (1 := (C, PrimSet, HS)).
+        eapply zero_tau_step; eauto.
+        eauto.
+        eapply Hp; eauto.
+      }
+    }
+  }
 
 Lemma wp_sim_ensures_refinement' :
   forall C Cas S pc npc PrimSet HS B idx,
